02_Earleys_Algorithm.thy
@@ -8,6 +8,9 @@ begin
 (*<*)
 syntax
   "length" :: "'a list \<Rightarrow> nat"  ("|_|")
+
+syntax
+  "card" ::  "'a set \<Rightarrow> nat" ("|_|")
 (*>*)
 
 chapter \<open>Earley's Recognizer \label{chapter:2}\<close>
